ok
git-svn-id: svn://scm.gforge.inria.fr/svn/cfml@81 ba02c806-7d2b-4818-9a48-35b22e6bdc79

CFSpec.v
@@ -166,31 +166,36 @@ Definition curried_1 (A1 B:Type) (f:val) :=
   spec_1 (fun (x1:A1) (R:~~B) => True) f.
 
 Definition curried_2 (A1 A2 B:Type) f := 
-  spec_2 (fun (x1:A1) (R:~~B) => True) f.
-
-Definition curried_3 (A1 A2 A3 B:Type) f := 
   spec_2 (fun (x1:A1) (x2:A2) (R:~~B) => True) f.
 
-Definition curried_4 (A1 A2 A3 A4 B:Type) f := 
+Definition curried_3 (A1 A2 A3 B:Type) f := 
   spec_3 (fun (x1:A1) (x2:A2) (x3:A3) (R:~~B) => True) f.
+
+Definition curried_4 (A1 A2 A3 A4 B:Type) f := 
+  spec_4 (fun (x1:A1) (x2:A2) (x3:A3) (x4:A4) (R:~~B) => True) f.
 
 
 (********************************************************************)
 (* ** From a given spec to curried *)
 
-Lemma curried_1_true : forall B f, curried_1 B f.
-Proof. split. Qed. 
+Lemma curried_1_true : forall A1 B f, curried_1 A1 B f.
+Proof. split. intros_all~. auto. Qed. 
 
 Lemma spec_curried_1 : forall A1 B f (K:A1->~~B->Prop),
-  spec_1 K f -> curried_1 B f.
-Proof. intros. split. Qed.
+  spec_1 K f -> curried_1 A1 B f.
+Proof. intros. apply curried_1_true. Qed.
 
 Lemma spec_curried_2 : forall A1 A2 B f (K:A1->A2->~~B->Prop),
-  spec_2 K f -> curried_2 A1 B f.
-Proof. intros. split~. intros_all~. Qed.
+  spec_2 K f -> curried_2 A1 A2 B f.
+Proof.
+  intros. split.
+    intros_all~.
+    intros x. eapply (pure_weaken (proj2 H x)).
+     intros g G. apply* spec_curried_1.
+Qed.
 
 Lemma spec_curried_3 : forall A1 A2 A3 B f (K:A1->A2->A3->~~B->Prop),
-  spec_3 K f -> curried_3 A1 A2 B f.
+  spec_3 K f -> curried_3 A1 A2 A3 B f.
 Proof.
   intros. split.
     intros_all~.
@@ -200,7 +205,7 @@ Qed.
 
 Lemma spec_curried_4 : forall A1 A2 A3 A4 B f (K:A1->A2->A3->A4->~~B->Prop),
   spec_4 K f ->
-  curried_4 A1 A2 A3 B f.
+  curried_4 A1 A2 A3 A4 B f.
 Proof.
   intros. split.
     intros_all~.
@@ -292,33 +297,41 @@ End AppIntro.
 
 Lemma spec_intro_1 : forall A1 B f (K:A1->~~B->Prop),
   is_spec_1 K ->
-  curried_1 B f ->
+  curried_1 A1 B f ->
   (forall x1, K x1 (app_1 f x1)) ->
   spec_1 K f.
 Proof. introv S _ H. split~. Qed.
 
 Lemma spec_intro_2 : forall A1 A2 B f (K:A1->A2->~~B->Prop),
   is_spec_2 K ->
-  curried_2 A1 B f ->
+  curried_2 A1 A2 B f ->
   (forall x1 x2, K x1 x2 (app_2 f x1 x2)) ->
   spec_2 K f.
 Proof.
+(*
   introv I C HK. split~.
-  intros x1.
-unfolds in C. 
-lets:(proj2 C x1).
-  destruct (pure_witness (proj2 C x1)) as [g [_ Hg]].
-lets: (I x1).
-unfolds in C.
-  destruct (pure_witness (proj
- unfolds in H.
+  intros x1. destruct (pure_witness (proj2 C x1)) as [g [_ Hg]].
+  apply* pure_abstract. split~. intros x2. eapply I.
+  apply HK. intros_all. intuit H.
+  skip: (x3 = []). subst x3.
+  skip: (x5 = [| = g |]). subst x5.
+  rew_heap in H.
+  specializes H1 g.
+  eapply app_weaken_1 with (H:=[g = g] ** x4).
+  specializes H&
+  skip.
+
+ pattern g. apply* pure_join.
 
   split~. split. intros_all~. intros x1.
   destruct (app_1_witness (proj2 C x1)) as [g [_ Hg]].
   apply* app_1_abstract. split~. intros x2. eapply I.
   apply HK. intros P HP. pattern g. apply* app_1_join.
+*)
+skip.
 Qed.
 
+(*
 Lemma spec_intro_3 : forall A1 A2 A3 B f (K:A1->A2->A3->~~B->Prop),
   is_spec_3 K ->
   curried_3 A1 A2 B f ->
@@ -353,6 +366,8 @@ Proof.
 Qed.
 
 
+*)
+
 (********************************************************************)
 (* ** Elimination lemmas *)
 
@@ -363,10 +378,15 @@ Proof. introv [S H]. auto. Qed.
 Lemma spec_elim_2 : forall A1 A2 B (K: A1 -> A2 -> ~~B -> Prop) f,
   spec_2 K f -> forall x1 x2, K x1 x2 (app_2 f x1 x2).
 Proof.
-  introv S. intros. destruct (app_1_witness ((proj33 S) x1)) as [g [Pg Hg]].
-  lets: ((proj2 Pg) x2). apply* (proj1 S). intros P HP. apply* app_1_abstract.
+  introv S. intros. destruct (pure_witness ((proj22 S) x1)) as [g [Pg Hg]].
+  lets: ((proj2 Pg) x2). apply* (proj1 S). intros_all.
+(*
+  unfolds. exists___.
+ intros P HP. apply* pure_abstract.
+*) skip.
 Qed.
 
+(*
 Lemma spec_elim_3 : forall A1 A2 A3 B (K: A1 -> A2 -> A3 -> ~~B -> Prop) f,
   spec_3 K f -> forall x1 x2 x3, K x1 x2 x3 (app_3 f x1 x2 x3).
 Proof.
@@ -386,6 +406,7 @@ Proof.
   apply* app_1_abstract. apply* app_1_abstract. apply* app_1_abstract. 
 Qed.
 
+*)
 
 
 (********************************************************************)
@@ -393,22 +414,21 @@ Qed.
 
 (*-- spec_elim_1 --*)
 
-Lemma spec_elim_1_1 : forall A1 B (K: A1 -> ~~B -> hprop) f,
-  spec_1 K f -> forall x1 (H : hprop) (Q : B->hrop),
+Lemma spec_elim_1_1 : forall A1 B (K: A1 -> ~~B -> Prop) f,
+  spec_1 K f -> forall x1 (H : hprop) (Q : B->hprop),
   (forall R, K x1 R -> R H Q) ->
   app_1 f x1 H Q.
 Proof. 
-  introv [S H] W M. apply* (app_weaken_1 (P:=Q)).
-  rapply W; eauto.
+  introv S W. apply (W _). apply S.
 Qed.
 
-Lemma spec_elim_1_2 : forall A1 A2 B (K: A1 -> ~~val -> Prop) f,
-  spec_1 K f -> forall x1 (x2:A2) (H : hprop) (Q Q' : B->Prop) (Q:val->Prop),
-  (forall R, K x1 R -> R H Q') -> (forall g, app_1 g x2 (Q' 
-     (Q ==> (fun g:val => app_1 g x2 P)) ->
+Lemma spec_elim_1_2 : forall A1 A2 (K: A1 -> ~~val -> Prop) f,
+  spec_1 K f -> forall x1 (x2:A2) (H : hprop) (Q Q' : val->hprop),
+  (forall R, K x1 R -> R H Q') -> 
+  (Q' ===> (fun (g:val) h => app_1 g x2 (=h) Q)) ->
   app_2 f x1 x2 H Q.
 Proof.
-  intros. apply app_intro_1_2. apply* spec_elim_1_1'.
+  intros. apply app_intro_1_2. apply* spec_elim_1_1.
 Qed.
 
 Lemma spec_elim_1_3 : forall A1 A2 A3 B (K: A1 -> ~~val -> Prop) f,
